Stored predicates and wrappers: cleanups
- eq -> Heq
- Better argument order for hoEnvD_inst (ease marking as NonExpansive).
- more consistent proofs for wrapper lemmas.

theories/dlang.v
@@ -63,10 +63,11 @@ Module Type LiftWp (Import VS : VlSortsSig).
     s n (φ : hoEnvD Σ n) := (∃ γ, (s ↦ γ) ∗ γ ⤇n[ n ] φ)%I.
   Notation "s ↝n[ n  ] φ" := (stamp_to_type_n s n φ) (at level 20) : bi_scope.
 
-  Definition hoEnvD_inst {n Σ} (φ : hoEnvD Σ n) σ : hoD Σ n := λ args, φ args (to_subst σ).
+  Program Definition hoEnvD_inst {i Σ} σ : hoEnvD Σ i -n> hoD Σ i := λne φ, λ args, φ args (to_subst σ).
+  Next Obligation. move => i Σ σ n x y Heq args. exact: Heq. Qed.
 
   Definition stamp_σ_to_type_n `{!dlangG Σ} s σ n (ψ : hoD Σ n) : iProp Σ :=
-    (∃ φ : hoEnvD Σ n, s ↝n[ n ] φ ∗ ▷ (ψ ≡ hoEnvD_inst φ σ))%I.
+    (∃ φ : hoEnvD Σ n, s ↝n[ n ] φ ∗ ▷ (ψ ≡ hoEnvD_inst σ φ))%I.
   Notation "s ↗n[ σ , n  ] ψ" := (stamp_σ_to_type_n s σ n ψ) (at level 20): bi_scope.
 
   Notation "γ ⤇ φ" := (γ ⤇n[ 0 ] vopen φ) (at level 20).
@@ -86,65 +87,66 @@ Module Type LiftWp (Import VS : VlSortsSig).
 
     Import EqNotations.
     Lemma stamp_to_type_agree_dep_abs {s n1 n2 φ1 φ2} :
-      s ↝n[ n1 ] φ1 -∗ s ↝n[ n2 ] φ2 -∗ ∃ eq : n1 = n2,
-        ▷ ((rew [hoEnvD Σ] eq in φ1) ≡ φ2).
+      s ↝n[ n1 ] φ1 -∗ s ↝n[ n2 ] φ2 -∗ ∃ Heq : n1 = n2,
+        ▷ ((rew [hoEnvD Σ] Heq in φ1) ≡ φ2).
     Proof.
       iDestruct 1 as (γ1) "[Hs1 Hg1]"; iDestruct 1 as (γ2) "[Hs2 Hg2]".
       iDestruct (mapsto_agree with "Hs1 Hs2") as %->.
-      iDestruct (saved_ho_sem_type_agree_dep_abs _ with "Hg1 Hg2") as (->) "Hgoal".
-      iExists eq_refl; simpl. by [].
+      iDestruct (saved_ho_sem_type_agree_dep_abs with "Hg1 Hg2") as (->) "Hgoal".
+      by iExists eq_refl.
     Qed.
 
     Lemma stamp_to_type_agree_dep {s n1 n2 φ1 φ2} args ρ v :
-      s ↝n[ n1 ] φ1 -∗ s ↝n[ n2 ] φ2 -∗ ∃ eq : n1 = n2,
-        ▷ ((rew [hoEnvD Σ] eq in φ1) args ρ v ≡ φ2 args ρ v).
+      s ↝n[ n1 ] φ1 -∗ s ↝n[ n2 ] φ2 -∗ ∃ Heq : n1 = n2,
+        ▷ ((rew [hoEnvD Σ] Heq in φ1) args ρ v ≡ φ2 args ρ v).
     Proof.
       iIntros "Hsg1 Hsg2".
-      iDestruct (stamp_to_type_agree_dep_abs with "Hsg1 Hsg2") as (->) "H".
-      iExists eq_refl; cbn.
-      iNext. repeat setoid_rewrite bi.discrete_fun_equivI. iApply "H".
+      iDestruct (stamp_to_type_agree_dep_abs with "Hsg1 Hsg2") as (->) "Hgoal".
+      iExists eq_refl; cbn. iNext.
+      by repeat setoid_rewrite bi.discrete_fun_equivI.
     Qed.
 
     Lemma stamp_to_type_agree {s n φ1 φ2} args ρ v :
       s ↝n[ n ] φ1 -∗ s ↝n[ n ] φ2 -∗ ▷ (φ1 args ρ v ≡ φ2 args ρ v).
     Proof.
       iIntros "Hs1 Hs2".
-      iDestruct (stamp_to_type_agree_dep args ρ v with "Hs1 Hs2") as (eq) "Hgoal".
-      rewrite (proof_irrel eq eq_refl) /=. by [].
+      iDestruct (stamp_to_type_agree_dep args ρ v with "Hs1 Hs2") as (Heq) "Hgoal".
+      by rewrite (proof_irrel Heq eq_refl) /=.
     Qed.
     (* Global Opaque stamp_to_type_n. *)
 
     Lemma stamp_σ_to_type_agree_dep_abs {σ s n1 n2 ψ1 ψ2} :
-      s ↗n[ σ , n1 ] ψ1 -∗ s ↗n[ σ , n2 ] ψ2 -∗ ∃ eq : n1 = n2,
-        ▷ ((rew [hoD Σ] eq in ψ1) ≡ ψ2).
+      s ↗n[ σ , n1 ] ψ1 -∗ s ↗n[ σ , n2 ] ψ2 -∗ ∃ Heq : n1 = n2,
+        ▷ ((rew [hoD Σ] Heq in ψ1) ≡ ψ2).
     Proof.
       iDestruct 1 as (φ1) "[Hsg1 Heq1]"; iDestruct 1 as (φ2) "[Hsg2 Heq2]".
       iDestruct (stamp_to_type_agree_dep_abs with "Hsg1 Hsg2") as (->) "Hgoal".
-      iExists eq_refl. iNext. cbn. iRewrite "Heq1"; iRewrite "Heq2".
+      iExists eq_refl. iNext.
+      iEval (cbn) in "Hgoal"; iEval (cbn). iRewrite "Heq1"; iRewrite "Heq2".
       repeat setoid_rewrite discrete_fun_equivI.
-      iIntros (??). iApply "Hgoal".
+      iIntros (??) "/=". iExact "Hgoal".
     Qed.
 
     Lemma stamp_σ_to_type_agree_dep {σ s n1 n2 ψ1 ψ2} args v :
-      s ↗n[ σ , n1 ] ψ1 -∗ s ↗n[ σ , n2 ] ψ2 -∗ ∃ eq : n1 = n2,
-        ▷ ((rew [hoD Σ] eq in ψ1) args v ≡ ψ2 args v).
+      s ↗n[ σ , n1 ] ψ1 -∗ s ↗n[ σ , n2 ] ψ2 -∗ ∃ Heq : n1 = n2,
+        ▷ ((rew [hoD Σ] Heq in ψ1) args v ≡ ψ2 args v).
     Proof.
       iIntros "H1 H2".
-      iDestruct (stamp_σ_to_type_agree_dep_abs with "H1 H2") as (->) "H".
-      iExists eq_refl; cbn. iNext.
-      repeat setoid_rewrite discrete_fun_equivI. iApply "H".
+      iDestruct (stamp_σ_to_type_agree_dep_abs with "H1 H2") as (->) "Hgoal".
+      iExists eq_refl; cbn; iNext.
+      by repeat setoid_rewrite discrete_fun_equivI.
     Qed.
 
     Lemma stamp_σ_to_type_agree {σ s n ψ1 ψ2} args v :
       s ↗n[ σ , n ] ψ1 -∗ s ↗n[ σ , n ] ψ2 -∗ ▷ (ψ1 args v ≡ ψ2 args v).
     Proof.
       iIntros "Hs1 Hs2".
-      iDestruct (stamp_σ_to_type_agree_dep args v with "Hs1 Hs2") as (eq) "H".
-      rewrite (proof_irrel eq eq_refl) /=. by [].
+      iDestruct (stamp_σ_to_type_agree_dep args v with "Hs1 Hs2") as (Heq) "H".
+      by rewrite (proof_irrel Heq eq_refl) /=.
     Qed.
 
     Lemma stamp_σ_to_type_intro s σ n (φ : hoEnvD Σ n) :
-      s ↝n[ n ] φ -∗ s ↗n[ σ , n ] hoEnvD_inst φ σ.
+      s ↝n[ n ] φ -∗ s ↗n[ σ , n ] hoEnvD_inst σ φ.
     Proof. rewrite /stamp_σ_to_type_n. iIntros; iExists φ; auto. Qed.
 
     Global Instance stamp_σ_to_type_persistent σ s n ψ : Persistent (s ↗n[ σ , n ] ψ) := _.
