theories/saved_interp_dep.v
@@ -112,52 +112,48 @@ Section saved_ho_sem_type.
     γ ⤇n[ i ] Φ1 -∗ γ ⤇n[ j ] Φ2 -∗ ⌜ i = j ⌝.
   Proof.
     iIntros "HΦ1 HΦ2".
-    (* iDestruct (packedHoEnvPred_arity_neI_pure with "[HΦ1 HΦ2]") as "?".
-    iApply (saved_anything_agree with "HΦ1 HΦ2"). done. *)
-    (* Fail iDestruct (packedHoEnvPred_arity_neI_pure $! (saved_anything_agree with "HΦ1 HΦ2")) as "?". *)
     iDestruct (saved_anything_agree with "HΦ1 HΦ2") as "Heq".
-    (* iDestruct (packedHoEnvPred_arity_neI_pure with "Heq") as "?". *)
-    rewrite packedHoEnvPred_arity_neI_pure. done.
+    by rewrite packedHoEnvPred_arity_neI_pure /=.
   Qed.
 
-  Lemma saved_ho_sem_type_agree_abs γ n (Φ1 Φ2 : hoEnvPred s Σ n):
-    γ ⤇n[ n ] Φ1 -∗ γ ⤇n[ n ] Φ2 -∗ ▷ (Φ1 ≡ Φ2).
+  Lemma saved_ho_sem_type_agree_dep_abs γ {i j Φ1 Φ2}:
+    γ ⤇n[ i ] Φ1 -∗ γ ⤇n[ j ] Φ2 -∗ ∃ Heq : i = j,
+    ▷ ((rew [hoEnvPred s Σ] Heq in Φ1) ≡ Φ2).
   Proof.
     iIntros "HΦ1 HΦ2".
+    iDestruct (saved_ho_sem_type_agree_arity with "HΦ1 HΦ2") as %->.
+    iExists eq_refl; cbn.
     iDestruct (saved_anything_agree with "HΦ1 HΦ2") as "Heq".
-    rewrite /= sigT_equivI. iDestruct "Heq" as (Heq) "Heq".
+    rewrite /= sigT_equivI. iDestruct "Heq" as (Heq) "Hgoal".
     rewrite (proof_irrel Heq eq_refl) /=.
-    repeat setoid_rewrite bi.discrete_fun_equivI; iNext.
-    iApply "Heq".
+    repeat setoid_rewrite bi.discrete_fun_equivI. by iNext.
+  Qed.
+
+  Lemma saved_ho_sem_type_agree_dep {γ i j Φ1 Φ2} a b c:
+    γ ⤇n[ i ] Φ1 -∗ γ ⤇n[ j ] Φ2 -∗ ∃ Heq : i = j,
+    ▷ ((rew [hoEnvPred s Σ] Heq in Φ1) a b c ≡ Φ2 a b c).
+  Proof.
+    iIntros "HΦ1 HΦ2".
+    iDestruct (saved_ho_sem_type_agree_dep_abs with "HΦ1 HΦ2") as (->) "Hgoal".
+    iExists eq_refl; cbn; iNext.
+    by repeat setoid_rewrite bi.discrete_fun_equivI.
   Qed.
 
   Lemma saved_ho_sem_type_agree γ n (Φ1 Φ2 : hoEnvPred s Σ n) a b c:
     γ ⤇n[ n ] Φ1 -∗ γ ⤇n[ n ] Φ2 -∗ ▷ (Φ1 a b c ≡ Φ2 a b c).
   Proof.
     iIntros "HΦ1 HΦ2".
-    iDestruct (saved_ho_sem_type_agree_abs with "HΦ1 HΦ2") as "H".
-    iNext. repeat setoid_rewrite bi.discrete_fun_equivI. iApply "H".
+    iDestruct (saved_ho_sem_type_agree_dep a b c with "HΦ1 HΦ2") as (Heq) "Hgoal".
+    by rewrite (proof_irrel Heq eq_refl) /=.
   Qed.
 
-  Lemma saved_ho_sem_type_agree_dep_abs γ {i j Φ1 Φ2}:
-    γ ⤇n[ i ] Φ1 -∗ γ ⤇n[ j ] Φ2 -∗ ∃ eq : i = j,
-    ▷ ((rew [hoEnvPred s Σ] eq in Φ1) ≡ Φ2).
+  (* Lemma saved_ho_sem_type_agree_abs γ n (Φ1 Φ2 : hoEnvPred s Σ n):
+    γ ⤇n[ n ] Φ1 -∗ γ ⤇n[ n ] Φ2 -∗ ▷ (Φ1 ≡ Φ2).
   Proof.
     iIntros "HΦ1 HΦ2".
-    iDestruct (saved_ho_sem_type_agree_arity with "HΦ1 HΦ2") as %->.
-    iExists eq_refl; cbn.
-    iApply (saved_ho_sem_type_agree_abs with "HΦ1 HΦ2").
-  Qed.
-
-  Lemma saved_ho_sem_type_agree_dep γ {i j Φ1 Φ2} a b c:
-    γ ⤇n[ i ] Φ1 -∗ γ ⤇n[ j ] Φ2 -∗ ∃ eq : i = j,
-    ▷ ((rew [hoEnvPred s Σ] eq in Φ1) a b c ≡ Φ2 a b c).
-  Proof.
-    iIntros "HΦ1 HΦ2".
-    iDestruct (saved_ho_sem_type_agree_dep_abs with "HΦ1 HΦ2") as (->) "H".
-    iExists eq_refl; iNext; simpl.
-    repeat setoid_rewrite bi.discrete_fun_equivI. iApply "H".
-  Qed.
+    iDestruct (saved_ho_sem_type_agree_dep_abs with "HΦ1 HΦ2") as (Heq) "Hgoal".
+    by rewrite (proof_irrel Heq eq_refl) /=.
+  Qed. *)
 End saved_ho_sem_type.
 
 Notation "γ ⤇n[ n  ] φ" := (saved_ho_sem_type_own γ n φ) (at level 20).
